<?xml version="1.0"?>
<rdf:RDF xmlns="http://ontology.ethereal.cz/irao#"
     xml:base="http://ontology.ethereal.cz/irao"
     xmlns:cc="http://web.resource.org/cc/"
     xmlns:dc="http://purl.org/dc/elements/1.1/"
     xmlns:ns="http://www.w3.org/2003/06/sw-vocab-status/ns#"
     xmlns:obo="http://purl.obolibrary.org/obo/"
     xmlns:owl="http://www.w3.org/2002/07/owl#"
     xmlns:rdf="http://www.w3.org/1999/02/22-rdf-syntax-ns#"
     xmlns:wot="http://xmlns.com/wot/0.1/"
     xmlns:xml="http://www.w3.org/XML/1998/namespace"
     xmlns:xsd="http://www.w3.org/2001/XMLSchema#"
     xmlns:dcam="http://purl.org/dc/dcam/"
     xmlns:foaf="http://xmlns.com/foaf/0.1/"
     xmlns:irao="http://ontology.ethereal.cz/irao/"
     xmlns:rdfs="http://www.w3.org/2000/01/rdf-schema#"
     xmlns:skos="http://www.w3.org/2004/02/skos/core#"
     xmlns:vann="http://purl.org/vocab/vann/"
     xmlns:skos1="http://www.w3.org/2008/05/skos#"
     xmlns:vitro="http://vitro.mannlib.cornell.edu/ns/vitro/0.7#"
     xmlns:dcterms="http://purl.org/dc/terms/"
     xmlns:statistics="http://purl.org/net/OCRe/statistics.owl#"
     xmlns:geopolitical="http://aims.fao.org/aos/geopolitical.owl#"
     xmlns:study_protocol="http://purl.org/net/OCRe/study_protocol.owl#">
    <owl:Ontology rdf:about="http://ontology.ethereal.cz/irao">
        <owl:versionIRI rdf:resource="https://w3id.org/def/InformaticsResearchArtifactsOntology"/>
        <!-- owl:imports rdf:resource="http://cso.kmi.open.ac.uk/schema/cso#"/ -->
        <!-- owl:imports rdf:resource="http://purl.org/dc/terms"/ -->
        <!-- owl:imports rdf:resource="http://purl.org/dc/elements/1.1"/ -->
        <!-- owl:imports rdf:resource="http://purl.org/vocab/vann/"/ -->
        <!-- owl:imports rdf:resource="http://vivoweb.org/ontology/core"/ -->
        <!-- owl:imports rdf:resource="http://xmlns.com/foaf/0.1/"/ -->
        <dc:contributor>Vojtěch Svátek</dc:contributor>
        <dc:creator>Nguyen Viet Bach</dc:creator>
        <dc:date rdf:datatype="http://www.w3.org/2001/XMLSchema#date">2021-03-18</dc:date>
        <dc:description xml:lang="en">Abstract: Informatics Research Artifacts Ontology, described using W3C RDF Schema and the Web Ontology Language OWL.</dc:description>
        <dc:publisher>Prague University of Economics and Business, Czech Republic. Faculty of Informatics and Statistics. Department of Knowledge and Information Engineering</dc:publisher>
        <dc:rights>Copyright © 2021 Prague University of Economics and Business</dc:rights>
        <dc:subject xml:lang="en">Informatics, Research Artifacts, Ontology, Semantic SEO, Linked Data, RDF, Semantic Web</dc:subject>
        <dc:title xml:lang="en">Informatics Research Artifacts Ontology</dc:title>
        <dcterms:abstract xml:lang="en">Abstract: Informatics Research Artifacts Ontology, described using W3C RDF Schema and the Web Ontology Language OWL.</dcterms:abstract>
        <dcterms:created rdf:datatype="http://www.w3.org/2001/XMLSchema#date">2021-03-18</dcterms:created>
        <dcterms:description xml:lang="en">Abstract: Informatics Research Artifacts Ontology, described using W3C RDF Schema and the Web Ontology Language OWL.</dcterms:description>
        <dcterms:license rdf:resource="https://creativecommons.org/licenses/by/3.0/"/>
        <dcterms:publisher>Prague University of Economics and Business, Czech Republic. Faculty of Informatics and Statistics. Department of Knowledge and Information Engineering</dcterms:publisher>
        <vann:preferredNamespacePrefix>irao</vann:preferredNamespacePrefix>
        <vann:preferredNamespaceUri>http://ontology.ethereal.cz/irao/</vann:preferredNamespaceUri>
        <rdfs:comment xml:lang="en">Abstract: Informatics Research Artifacts Ontology, described using W3C RDF Schema and the Web Ontology Language OWL.</rdfs:comment>
        <rdfs:label xml:lang="en">Informatics Research Artifacts Ontology</rdfs:label>
        <owl:versionInfo xml:lang="en">Version 1.1.1, Release 2021 Mar 18</owl:versionInfo>
    </owl:Ontology>
    


    <!-- 
    ///////////////////////////////////////////////////////////////////////////////////////
    //
    // Object Properties
    //
    ///////////////////////////////////////////////////////////////////////////////////////
     -->

    


    <!-- http://ontology.ethereal.cz/irao/hasAccessibility -->

    <owl:ObjectProperty rdf:about="http://ontology.ethereal.cz/irao/hasAccessibility">
        <rdfs:domain rdf:resource="http://ontology.ethereal.cz/irao/ResearchArtifact"/>
        <rdfs:range rdf:resource="http://ontology.ethereal.cz/irao/Accessibility"/>
        <rdfs:comment xml:lang="en">This property specifies the accessibility of a research artifact</rdfs:comment>
        <rdfs:isDefinedBy rdf:resource="http://ontology.ethereal.cz/irao"/>
        <rdfs:label xml:lang="en">has accessibility</rdfs:label>
    </owl:ObjectProperty>
    


    <!-- http://ontology.ethereal.cz/irao/hasAffiliation -->

    <owl:ObjectProperty rdf:about="http://ontology.ethereal.cz/irao/hasAffiliation">
        <rdfs:domain rdf:resource="http://ontology.ethereal.cz/irao/Researcher"/>
        <rdfs:range rdf:resource="http://ontology.ethereal.cz/irao/Affiliation"/>
        <rdfs:comment xml:lang="en">This property specifies the affiliation of a researcher</rdfs:comment>
        <rdfs:isDefinedBy rdf:resource="http://ontology.ethereal.cz/irao"/>
        <rdfs:label xml:lang="en">has affiliation</rdfs:label>
    </owl:ObjectProperty>
    


    <!-- http://ontology.ethereal.cz/irao/hasAuthor -->

    <owl:ObjectProperty rdf:about="http://ontology.ethereal.cz/irao/hasAuthor">
        <rdfs:domain rdf:resource="http://ontology.ethereal.cz/irao/ResearchArtifact"/>
        <rdfs:range rdf:resource="http://xmlns.com/foaf/0.1/Person"/>
        <rdfs:comment xml:lang="en">This property specifies the author of a research artifact</rdfs:comment>
        <rdfs:isDefinedBy rdf:resource="http://ontology.ethereal.cz/irao"/>
        <rdfs:label xml:lang="en">has author</rdfs:label>
    </owl:ObjectProperty>
    


    <!-- http://ontology.ethereal.cz/irao/hasDesign -->

    <owl:ObjectProperty rdf:about="http://ontology.ethereal.cz/irao/hasDesign">
        <rdfs:domain rdf:resource="http://ontology.ethereal.cz/irao/ResearchArtifact"/>
        <rdfs:range rdf:resource="http://ontology.ethereal.cz/irao/DesignQuality"/>
        <rdfs:comment xml:lang="en">This property specifies the design of a research artifact</rdfs:comment>
        <rdfs:isDefinedBy rdf:resource="http://ontology.ethereal.cz/irao"/>
        <rdfs:label xml:lang="en">has design</rdfs:label>
    </owl:ObjectProperty>
    


    <!-- http://ontology.ethereal.cz/irao/hasDesignQuality -->

    <owl:ObjectProperty rdf:about="http://ontology.ethereal.cz/irao/hasDesignQuality">
        <rdfs:domain rdf:resource="http://ontology.ethereal.cz/irao/Design"/>
        <rdfs:range rdf:resource="http://ontology.ethereal.cz/irao/DesignQuality"/>
        <rdfs:comment xml:lang="en">This property specifies the design quality of a design</rdfs:comment>
        <rdfs:isDefinedBy rdf:resource="http://ontology.ethereal.cz/irao"/>
        <rdfs:label xml:lang="en">has design quality</rdfs:label>
    </owl:ObjectProperty>
    


    <!-- http://ontology.ethereal.cz/irao/hasDevelopmentStatus -->

    <owl:ObjectProperty rdf:about="http://ontology.ethereal.cz/irao/hasDevelopmentStatus">
        <rdfs:domain rdf:resource="http://ontology.ethereal.cz/irao/ResearchArtifact"/>
        <rdfs:range rdf:resource="http://ontology.ethereal.cz/irao/DevelopmentStatus"/>
        <rdfs:comment xml:lang="en">This property specifies the development status of a research artifact</rdfs:comment>
        <rdfs:isDefinedBy rdf:resource="http://ontology.ethereal.cz/irao"/>
        <rdfs:label xml:lang="en">has development status</rdfs:label>
    </owl:ObjectProperty>
    


    <!-- http://ontology.ethereal.cz/irao/hasDomain -->

    <owl:ObjectProperty rdf:about="http://ontology.ethereal.cz/irao/hasDomain">
        <rdfs:domain rdf:resource="http://ontology.ethereal.cz/irao/ResearchArtifact"/>
        <rdfs:range rdf:resource="http://ontology.ethereal.cz/irao/ResearchDomain"/>
        <rdfs:comment xml:lang="en">This property specifies the research domain of a research artifact</rdfs:comment>
        <rdfs:isDefinedBy rdf:resource="http://ontology.ethereal.cz/irao"/>
        <rdfs:label xml:lang="en">has domain</rdfs:label>
    </owl:ObjectProperty>
    


    <!-- http://ontology.ethereal.cz/irao/hasField -->

    <owl:ObjectProperty rdf:about="http://ontology.ethereal.cz/irao/hasField">
        <rdfs:domain rdf:resource="http://ontology.ethereal.cz/irao/ResearchArtifact"/>
        <rdfs:range rdf:resource="http://ontology.ethereal.cz/irao/ResearchField"/>
        <rdfs:comment xml:lang="en">This property specifies the research field of a research artifact</rdfs:comment>
        <rdfs:isDefinedBy rdf:resource="http://ontology.ethereal.cz/irao"/>
        <rdfs:label xml:lang="en">has field</rdfs:label>
    </owl:ObjectProperty>
    


    <!-- http://ontology.ethereal.cz/irao/hasFollowedProtocol -->

    <owl:ObjectProperty rdf:about="http://ontology.ethereal.cz/irao/hasFollowedProtocol">
        <rdfs:domain rdf:resource="http://ontology.ethereal.cz/irao/Benchmark"/>
        <rdfs:range rdf:resource="http://ontology.ethereal.cz/irao/Protocol"/>
        <rdfs:comment xml:lang="en">This property specifies the protocol that a benchmark follows</rdfs:comment>
        <rdfs:isDefinedBy rdf:resource="http://ontology.ethereal.cz/irao"/>
        <rdfs:label xml:lang="en">has followed protocol</rdfs:label>
    </owl:ObjectProperty>
    


    <!-- http://ontology.ethereal.cz/irao/hasFramework -->

    <owl:ObjectProperty rdf:about="http://ontology.ethereal.cz/irao/hasFramework">
        <rdfs:domain rdf:resource="http://ontology.ethereal.cz/irao/Software"/>
        <rdfs:range rdf:resource="http://ontology.ethereal.cz/irao/Framework"/>
        <rdfs:comment xml:lang="en">This property specifies the framework used by a software</rdfs:comment>
        <rdfs:isDefinedBy rdf:resource="http://ontology.ethereal.cz/irao"/>
        <rdfs:label xml:lang="en">has framework</rdfs:label>
    </owl:ObjectProperty>
    


    <!-- http://ontology.ethereal.cz/irao/hasLicense -->

    <owl:ObjectProperty rdf:about="http://ontology.ethereal.cz/irao/hasLicense">
        <rdfs:domain rdf:resource="http://ontology.ethereal.cz/irao/ResearchArtifact"/>
        <rdfs:range rdf:resource="http://ontology.ethereal.cz/irao/License"/>
        <rdfs:comment xml:lang="en">This property specifies the license of a research artifact</rdfs:comment>
        <rdfs:isDefinedBy rdf:resource="http://ontology.ethereal.cz/irao"/>
        <rdfs:label xml:lang="en">has license</rdfs:label>
    </owl:ObjectProperty>
    


    <!-- http://ontology.ethereal.cz/irao/hasLicenseType -->

    <owl:ObjectProperty rdf:about="http://ontology.ethereal.cz/irao/hasLicenseType">
        <rdfs:domain rdf:resource="http://ontology.ethereal.cz/irao/License"/>
        <rdfs:range rdf:resource="http://ontology.ethereal.cz/irao/LicenseType"/>
        <rdfs:comment xml:lang="en">This property specifies the type of a license</rdfs:comment>
        <rdfs:isDefinedBy rdf:resource="http://ontology.ethereal.cz/irao"/>
        <rdfs:label xml:lang="en">has license type</rdfs:label>
    </owl:ObjectProperty>
    


    <!-- http://ontology.ethereal.cz/irao/hasMeasuringSystem -->

    <owl:ObjectProperty rdf:about="http://ontology.ethereal.cz/irao/hasMeasuringSystem">
        <rdfs:domain rdf:resource="http://ontology.ethereal.cz/irao/Benchmark"/>
        <rdfs:range rdf:resource="http://ontology.ethereal.cz/irao/System"/>
        <rdfs:comment xml:lang="en">This property specifies a system that measures a benchmark</rdfs:comment>
        <rdfs:isDefinedBy rdf:resource="http://ontology.ethereal.cz/irao"/>
        <rdfs:label xml:lang="en">has measuring system</rdfs:label>
    </owl:ObjectProperty>
    


    <!-- http://ontology.ethereal.cz/irao/hasMethodology -->

    <owl:ObjectProperty rdf:about="http://ontology.ethereal.cz/irao/hasMethodology">
        <rdfs:domain>
            <owl:Class>
                <owl:unionOf rdf:parseType="Collection">
                    <rdf:Description rdf:about="http://ontology.ethereal.cz/irao/Dataset"/>
                    <rdf:Description rdf:about="http://ontology.ethereal.cz/irao/Framework"/>
                    <rdf:Description rdf:about="http://ontology.ethereal.cz/irao/Protocol"/>
                </owl:unionOf>
            </owl:Class>
        </rdfs:domain>
        <rdfs:range rdf:resource="http://ontology.ethereal.cz/irao/Methodology"/>
        <rdfs:comment xml:lang="en">This property specifies the methodology used by a research artifact</rdfs:comment>
        <rdfs:isDefinedBy rdf:resource="http://ontology.ethereal.cz/irao"/>
        <rdfs:label xml:lang="en">has methodology</rdfs:label>
    </owl:ObjectProperty>
    


    <!-- http://ontology.ethereal.cz/irao/hasOpenStandard -->

    <owl:ObjectProperty rdf:about="http://ontology.ethereal.cz/irao/hasOpenStandard">
        <rdfs:domain rdf:resource="http://ontology.ethereal.cz/irao/ResearchArtifact"/>
        <rdfs:range rdf:resource="http://ontology.ethereal.cz/irao/OpenStandard"/>
        <rdfs:comment xml:lang="en">This property specifies the open standard used by a research artifact</rdfs:comment>
        <rdfs:isDefinedBy rdf:resource="http://ontology.ethereal.cz/irao"/>
        <rdfs:label xml:lang="en">has open standard</rdfs:label>
    </owl:ObjectProperty>
    


    <!-- http://ontology.ethereal.cz/irao/hasProducedDataset -->

    <owl:ObjectProperty rdf:about="http://ontology.ethereal.cz/irao/hasProducedDataset">
        <rdfs:domain rdf:resource="http://ontology.ethereal.cz/irao/Benchmark"/>
        <rdfs:range rdf:resource="http://ontology.ethereal.cz/irao/Dataset"/>
        <rdfs:comment xml:lang="en">This property specifies the dataset which us produced by a benchmark</rdfs:comment>
        <rdfs:isDefinedBy rdf:resource="http://ontology.ethereal.cz/irao"/>
        <rdfs:label xml:lang="en">has produced dataset</rdfs:label>
    </owl:ObjectProperty>
    


    <!-- http://ontology.ethereal.cz/irao/hasPublication -->

    <owl:ObjectProperty rdf:about="http://ontology.ethereal.cz/irao/hasPublication">
        <rdfs:domain rdf:resource="http://ontology.ethereal.cz/irao/ResearchArtifact"/>
        <rdfs:range rdf:resource="http://ontology.ethereal.cz/irao/Publication"/>
        <rdfs:comment xml:lang="en">This property specifies the publication of a research artifact</rdfs:comment>
        <rdfs:isDefinedBy rdf:resource="http://ontology.ethereal.cz/irao"/>
        <rdfs:label xml:lang="en">has publication</rdfs:label>
    </owl:ObjectProperty>
    


    <!-- http://ontology.ethereal.cz/irao/hasReferredBenchmark -->

    <owl:ObjectProperty rdf:about="http://ontology.ethereal.cz/irao/hasReferredBenchmark">
        <rdfs:domain rdf:resource="http://ontology.ethereal.cz/irao/Benchmark"/>
        <rdfs:range rdf:resource="http://ontology.ethereal.cz/irao/Benchmark"/>
        <rdfs:comment xml:lang="en">This property specifies a benchmark referred by another benchmark</rdfs:comment>
        <rdfs:isDefinedBy rdf:resource="http://ontology.ethereal.cz/irao"/>
        <rdfs:label xml:lang="en">has referred benchmark</rdfs:label>
    </owl:ObjectProperty>
    


    <!-- http://ontology.ethereal.cz/irao/hasRepositoryType -->

    <owl:ObjectProperty rdf:about="http://ontology.ethereal.cz/irao/hasRepositoryType">
        <rdfs:domain rdf:resource="http://ontology.ethereal.cz/irao/Repository"/>
        <rdfs:range rdf:resource="http://ontology.ethereal.cz/irao/RepositoryType"/>
        <rdfs:comment xml:lang="en">This property specifies the repository type of a research artifact repository</rdfs:comment>
        <rdfs:isDefinedBy rdf:resource="http://ontology.ethereal.cz/irao"/>
        <rdfs:label xml:lang="en">has repository type</rdfs:label>
    </owl:ObjectProperty>
    


    <!-- http://ontology.ethereal.cz/irao/hasResearchArea -->

    <owl:ObjectProperty rdf:about="http://ontology.ethereal.cz/irao/hasResearchArea">
        <rdfs:domain rdf:resource="http://ontology.ethereal.cz/irao/ResearchArtifact"/>
        <rdfs:range rdf:resource="http://cso.kmi.open.ac.uk/schema/cso#Topic"/>
        <rdfs:comment xml:lang="en">This property specifies the research area of a research artifact</rdfs:comment>
        <rdfs:isDefinedBy rdf:resource="http://ontology.ethereal.cz/irao"/>
        <rdfs:label xml:lang="en">has research area</rdfs:label>
    </owl:ObjectProperty>
    


    <!-- http://ontology.ethereal.cz/irao/hasResearchOutput -->

    <owl:ObjectProperty rdf:about="http://ontology.ethereal.cz/irao/hasResearchOutput">
        <rdfs:domain rdf:resource="http://ontology.ethereal.cz/irao/ResearchProject"/>
        <rdfs:range rdf:resource="http://ontology.ethereal.cz/irao/ResearchOutput"/>
        <rdfs:comment xml:lang="en">This property specifies the research output of a research project</rdfs:comment>
        <rdfs:isDefinedBy rdf:resource="http://ontology.ethereal.cz/irao"/>
        <rdfs:label xml:lang="en">has research output</rdfs:label>
    </owl:ObjectProperty>
    


    <!-- http://ontology.ethereal.cz/irao/hasUsedFramework -->

    <owl:ObjectProperty rdf:about="http://ontology.ethereal.cz/irao/hasUsedFramework">
        <rdfs:domain>
            <owl:Class>
                <owl:unionOf rdf:parseType="Collection">
                    <rdf:Description rdf:about="http://ontology.ethereal.cz/irao/Framework"/>
                    <rdf:Description rdf:about="http://ontology.ethereal.cz/irao/Software"/>
                    <rdf:Description rdf:about="http://ontology.ethereal.cz/irao/System"/>
                </owl:unionOf>
            </owl:Class>
        </rdfs:domain>
        <rdfs:range rdf:resource="http://ontology.ethereal.cz/irao/Framework"/>
        <rdfs:comment xml:lang="en">This property specifies the framework used by a research artifact like software or system</rdfs:comment>
        <rdfs:isDefinedBy rdf:resource="http://ontology.ethereal.cz/irao"/>
        <rdfs:label xml:lang="en">has used framework</rdfs:label>
    </owl:ObjectProperty>
    


    <!-- http://ontology.ethereal.cz/irao/hasUsedMethodology -->

    <owl:ObjectProperty rdf:about="http://ontology.ethereal.cz/irao/hasUsedMethodology">
        <rdfs:domain>
            <owl:Class>
                <owl:unionOf rdf:parseType="Collection">
                    <rdf:Description rdf:about="http://ontology.ethereal.cz/irao/Dataset"/>
                    <rdf:Description rdf:about="http://ontology.ethereal.cz/irao/Framework"/>
                </owl:unionOf>
            </owl:Class>
        </rdfs:domain>
        <rdfs:range rdf:resource="http://ontology.ethereal.cz/irao/Methodology"/>
        <rdfs:comment xml:lang="en">This property specifies the methodology used in a research artifact like framework or dataset</rdfs:comment>
        <rdfs:isDefinedBy rdf:resource="http://ontology.ethereal.cz/irao"/>
        <rdfs:label xml:lang="en">has used methodology</rdfs:label>
    </owl:ObjectProperty>
    


    <!-- http://ontology.ethereal.cz/irao/hasUsedOntologyDesignPattern -->

    <owl:ObjectProperty rdf:about="http://ontology.ethereal.cz/irao/hasUsedOntologyDesignPattern">
        <rdfs:domain>
            <owl:Class>
                <owl:unionOf rdf:parseType="Collection">
                    <rdf:Description rdf:about="http://ontology.ethereal.cz/irao/Ontology"/>
                    <rdf:Description rdf:about="http://ontology.ethereal.cz/irao/OntologyDesignPattern"/>
                </owl:unionOf>
            </owl:Class>
        </rdfs:domain>
        <rdfs:range rdf:resource="http://ontology.ethereal.cz/irao/OntologyDesignPattern"/>
        <rdfs:comment xml:lang="en">This property specifies the ontology design pattern of an ontology or another ontology design pattern</rdfs:comment>
        <rdfs:isDefinedBy rdf:resource="http://ontology.ethereal.cz/irao"/>
        <rdfs:label xml:lang="en">has used ontology design pattern</rdfs:label>
    </owl:ObjectProperty>
    


    <!-- http://ontology.ethereal.cz/irao/isDescribedBy -->

    <owl:ObjectProperty rdf:about="http://ontology.ethereal.cz/irao/isDescribedBy">
        <rdfs:domain rdf:resource="http://ontology.ethereal.cz/irao/Dataset"/>
        <rdfs:range rdf:resource="http://ontology.ethereal.cz/irao/DataModel"/>
        <rdfs:comment xml:lang="en">This property specifies the data model of a dataset</rdfs:comment>
        <rdfs:isDefinedBy rdf:resource="http://ontology.ethereal.cz/irao"/>
        <rdfs:label xml:lang="en">is described by</rdfs:label>
    </owl:ObjectProperty>
    


    <!-- http://ontology.ethereal.cz/irao/isFollowedBy -->

    <owl:ObjectProperty rdf:about="http://ontology.ethereal.cz/irao/isFollowedBy">
        <rdfs:domain rdf:resource="http://ontology.ethereal.cz/irao/ResearchProject"/>
        <rdfs:range rdf:resource="http://ontology.ethereal.cz/irao/ResearchProject"/>
        <rdfs:comment xml:lang="en">This property specifies that a research project is followed by another research project</rdfs:comment>
        <rdfs:isDefinedBy rdf:resource="http://ontology.ethereal.cz/irao"/>
        <rdfs:label xml:lang="en">is followed by</rdfs:label>
    </owl:ObjectProperty>
    


    <!-- http://ontology.ethereal.cz/irao/hasMaintainer -->

    <owl:ObjectProperty rdf:about="http://ontology.ethereal.cz/irao/hasMaintainer">
        <rdfs:domain rdf:resource="http://ontology.ethereal.cz/irao/ResearchArtifact"/>
        <rdfs:range rdf:resource="http://ontology.ethereal.cz/irao/Researcher"/>
        <rdfs:comment xml:lang="en">This property specifies the maintainer of a research artifact</rdfs:comment>
        <rdfs:isDefinedBy rdf:resource="http://ontology.ethereal.cz/irao"/>
        <rdfs:label xml:lang="en">is maintained by</rdfs:label>
    </owl:ObjectProperty>
    


    <!-- http://ontology.ethereal.cz/irao/isPartOfSystem -->

    <owl:ObjectProperty rdf:about="http://ontology.ethereal.cz/irao/isPartOfSystem">
        <rdfs:domain rdf:resource="http://ontology.ethereal.cz/irao/Software"/>
        <rdfs:range rdf:resource="http://ontology.ethereal.cz/irao/System"/>
        <rdfs:comment xml:lang="en">This property specifies the system which a software is part of</rdfs:comment>
        <rdfs:isDefinedBy rdf:resource="http://ontology.ethereal.cz/irao"/>
        <rdfs:label xml:lang="en">is part of system</rdfs:label>
    </owl:ObjectProperty>
    


    <!-- http://ontology.ethereal.cz/irao/isPublishedAt -->

    <owl:ObjectProperty rdf:about="http://ontology.ethereal.cz/irao/isPublishedAt">
        <rdfs:domain rdf:resource="http://ontology.ethereal.cz/irao/ResearchArtifact"/>
        <rdfs:range rdf:resource="http://ontology.ethereal.cz/irao/Repository"/>
        <rdfs:comment xml:lang="en">This property specifies the repository that a research artifact is published at</rdfs:comment>
        <rdfs:isDefinedBy rdf:resource="http://ontology.ethereal.cz/irao"/>
        <rdfs:label xml:lang="en">is published at</rdfs:label>
    </owl:ObjectProperty>
    


    <!-- http://ontology.ethereal.cz/irao/isUsedBy -->

    <owl:ObjectProperty rdf:about="http://ontology.ethereal.cz/irao/isUsedBy">
        <rdfs:domain rdf:resource="http://ontology.ethereal.cz/irao/ResearchArtifact"/>
        <rdfs:range rdf:resource="http://ontology.ethereal.cz/irao/ResearchArtifact"/>
        <rdfs:comment xml:lang="en">This property specifies that a research artifact is used by another research artifact</rdfs:comment>
        <rdfs:isDefinedBy rdf:resource="http://ontology.ethereal.cz/irao"/>
        <rdfs:label xml:lang="en">is used by</rdfs:label>
    </owl:ObjectProperty>
    


    <!-- 
    ///////////////////////////////////////////////////////////////////////////////////////
    //
    // Data properties
    //
    ///////////////////////////////////////////////////////////////////////////////////////
     -->

    


    <!-- http://ontology.ethereal.cz/irao/hasTopic -->

    <owl:DatatypeProperty rdf:about="http://ontology.ethereal.cz/irao/hasTopic">
        <rdfs:domain rdf:resource="http://ontology.ethereal.cz/irao/Publication"/>
        <rdfs:range rdf:resource="http://www.w3.org/2001/XMLSchema#string"/>
        <rdfs:comment xml:lang="en">This property specifies the topic of a publication</rdfs:comment>
        <rdfs:isDefinedBy rdf:resource="http://ontology.ethereal.cz/irao"/>
        <rdfs:label xml:lang="en">has topic</rdfs:label>
    </owl:DatatypeProperty>
    


    <!-- http://ontology.ethereal.cz/irao/hasURL -->

    <owl:DatatypeProperty rdf:about="http://ontology.ethereal.cz/irao/hasURL">
        <rdfs:domain>
            <owl:Class>
                <owl:unionOf rdf:parseType="Collection">
                    <rdf:Description rdf:about="http://ontology.ethereal.cz/irao/Publication"/>
                    <rdf:Description rdf:about="http://ontology.ethereal.cz/irao/Repository"/>
                    <rdf:Description rdf:about="http://ontology.ethereal.cz/irao/ResearchArtifact"/>
                </owl:unionOf>
            </owl:Class>
        </rdfs:domain>
        <rdfs:range rdf:resource="http://www.w3.org/2001/XMLSchema#anyURI"/>
        <rdfs:comment xml:lang="en">This property specifies the resource URL of a publication, repository or research artifact</rdfs:comment>
        <rdfs:isDefinedBy rdf:resource="http://ontology.ethereal.cz/irao"/>
        <rdfs:label xml:lang="en">has URL</rdfs:label>
    </owl:DatatypeProperty>
    


    <!-- http://ontology.ethereal.cz/irao/hasVersion -->

    <owl:DatatypeProperty rdf:about="http://ontology.ethereal.cz/irao/hasVersion">
        <rdfs:domain rdf:resource="http://ontology.ethereal.cz/irao/ResearchArtifact"/>
        <rdfs:range rdf:resource="http://www.w3.org/2001/XMLSchema#string"/>
        <rdfs:comment xml:lang="en">This property specifies the version of a research artifact</rdfs:comment>
        <rdfs:isDefinedBy rdf:resource="http://ontology.ethereal.cz/irao"/>
        <rdfs:label xml:lang="en">has version</rdfs:label>
    </owl:DatatypeProperty>
    


    <!-- 
    ///////////////////////////////////////////////////////////////////////////////////////
    //
    // Classes
    //
    ///////////////////////////////////////////////////////////////////////////////////////
     -->

    


    <!-- http://ontology.ethereal.cz/irao/API -->

    <owl:Class rdf:about="http://ontology.ethereal.cz/irao/API">
        <rdfs:subClassOf rdf:resource="http://ontology.ethereal.cz/irao/Service"/>
        <rdfs:comment xml:lang="en">An API is a type of service-based research artifact</rdfs:comment>
        <rdfs:isDefinedBy rdf:resource="http://ontology.ethereal.cz/irao"/>
        <rdfs:label xml:lang="en">API</rdfs:label>
    </owl:Class>
    


    <!-- http://ontology.ethereal.cz/irao/Accessibility -->

    <owl:Class rdf:about="http://ontology.ethereal.cz/irao/Accessibility">
        <rdfs:comment xml:lang="en">A research artifact can be made accessible via download or some kind of API, etc.</rdfs:comment>
        <rdfs:isDefinedBy rdf:resource="http://ontology.ethereal.cz/irao"/>
        <rdfs:label xml:lang="en">Accessibility</rdfs:label>
    </owl:Class>
    


    <!-- http://ontology.ethereal.cz/irao/Affiliation -->

    <owl:Class rdf:about="http://ontology.ethereal.cz/irao/Affiliation">
        <rdfs:comment xml:lang="en">An affiliation of the author, it maybe a company or an institution</rdfs:comment>
        <rdfs:isDefinedBy rdf:resource="http://ontology.ethereal.cz/irao"/>
        <rdfs:label xml:lang="en">Affiliation</rdfs:label>
    </owl:Class>
    


    <!-- http://ontology.ethereal.cz/irao/AnnotatedDataset -->

    <owl:Class rdf:about="http://ontology.ethereal.cz/irao/AnnotatedDataset">
        <rdfs:subClassOf rdf:resource="http://ontology.ethereal.cz/irao/Dataset"/>
        <rdfs:comment xml:lang="en">A dataset which was processed for AI or machine learning</rdfs:comment>
        <rdfs:isDefinedBy rdf:resource="http://ontology.ethereal.cz/irao"/>
        <rdfs:label xml:lang="en">Annotated Dataset</rdfs:label>
    </owl:Class>
    


    <!-- http://ontology.ethereal.cz/irao/ApplicationFramework -->

    <owl:Class rdf:about="http://ontology.ethereal.cz/irao/ApplicationFramework">
        <rdfs:subClassOf rdf:resource="http://ontology.ethereal.cz/irao/SoftwareFramework"/>
        <rdfs:comment xml:lang="en">A framework that is used by applications</rdfs:comment>
        <rdfs:isDefinedBy rdf:resource="http://ontology.ethereal.cz/irao"/>
        <rdfs:label xml:lang="en">Application Framework</rdfs:label>
    </owl:Class>
    


    <!-- http://ontology.ethereal.cz/irao/Benchmark -->

    <owl:Class rdf:about="http://ontology.ethereal.cz/irao/Benchmark">
        <rdfs:subClassOf rdf:resource="http://ontology.ethereal.cz/irao/InformaticsResearchArtifact"/>
        <rdfs:comment xml:lang="en">A benchmark is a type of comparison and measuring with metrics, producing datasets and algorithms for comprehensive and systematic evaluation of existing and future systems</rdfs:comment>
        <rdfs:isDefinedBy rdf:resource="http://ontology.ethereal.cz/irao"/>
        <rdfs:label xml:lang="en">Benchmark</rdfs:label>
    </owl:Class>
    


    <!-- http://ontology.ethereal.cz/irao/ConferencePaper -->

    <owl:Class rdf:about="http://ontology.ethereal.cz/irao/ConferencePaper">
        <rdfs:subClassOf rdf:resource="http://ontology.ethereal.cz/irao/Publication"/>
        <rdfs:comment xml:lang="en">A paper or article published at a scientific conference</rdfs:comment>
        <rdfs:isDefinedBy rdf:resource="http://ontology.ethereal.cz/irao"/>
        <rdfs:label xml:lang="en">Conference paper</rdfs:label>
    </owl:Class>
    


    <!-- http://ontology.ethereal.cz/irao/DataModel -->

    <owl:Class rdf:about="http://ontology.ethereal.cz/irao/DataModel">
        <rdfs:subClassOf rdf:resource="http://ontology.ethereal.cz/irao/Model"/>
        <rdfs:comment xml:lang="en">A data model such as schema and ontologies</rdfs:comment>
        <rdfs:isDefinedBy rdf:resource="http://ontology.ethereal.cz/irao"/>
        <rdfs:label xml:lang="en">Data model</rdfs:label>
    </owl:Class>
    


    <!-- http://ontology.ethereal.cz/irao/Dataset -->

    <owl:Class rdf:about="http://ontology.ethereal.cz/irao/Dataset">
        <rdfs:subClassOf rdf:resource="http://ontology.ethereal.cz/irao/InformaticsResearchArtifact"/>
        <rdfs:comment xml:lang="en">A dataset containing the gathered or generated data about some topic</rdfs:comment>
        <rdfs:isDefinedBy rdf:resource="http://ontology.ethereal.cz/irao"/>
        <rdfs:label xml:lang="en">Dataset</rdfs:label>
    </owl:Class>
    


    <!-- http://ontology.ethereal.cz/irao/Design -->

    <owl:Class rdf:about="http://ontology.ethereal.cz/irao/Design">
        <rdfs:subClassOf rdf:resource="http://ontology.ethereal.cz/irao/InformaticsResearchArtifact"/>
        <rdfs:comment xml:lang="en">A plan or specification for the construction or production of a research artifact</rdfs:comment>
        <rdfs:isDefinedBy rdf:resource="http://ontology.ethereal.cz/irao"/>
        <rdfs:label xml:lang="en">Design</rdfs:label>
    </owl:Class>
    


    <!-- http://ontology.ethereal.cz/irao/DesignQuality -->

    <owl:Class rdf:about="http://ontology.ethereal.cz/irao/DesignQuality">
        <rdfs:comment xml:lang="en">A design quality involves the usage of recommended standards, protocols, frameworks, methodologies</rdfs:comment>
        <rdfs:isDefinedBy rdf:resource="http://ontology.ethereal.cz/irao"/>
        <rdfs:label xml:lang="en">Design quality</rdfs:label>
    </owl:Class>
    


    <!-- http://ontology.ethereal.cz/irao/DevelopmentStatus -->

    <owl:Class rdf:about="http://ontology.ethereal.cz/irao/DevelopmentStatus">
        <rdfs:comment xml:lang="en">The development status of a research artifact, informing about its maturity</rdfs:comment>
        <rdfs:isDefinedBy rdf:resource="http://ontology.ethereal.cz/irao"/>
        <rdfs:label xml:lang="en">Development status</rdfs:label>
    </owl:Class>
    


    <!-- http://ontology.ethereal.cz/irao/Framework -->

    <owl:Class rdf:about="http://ontology.ethereal.cz/irao/Framework">
        <rdfs:subClassOf rdf:resource="http://ontology.ethereal.cz/irao/InformaticsResearchArtifact"/>
        <rdfs:comment xml:lang="en">The framework is a type of an informatics research artifact</rdfs:comment>
        <rdfs:isDefinedBy rdf:resource="http://ontology.ethereal.cz/irao"/>
        <rdfs:label xml:lang="en">Framework</rdfs:label>
    </owl:Class>
    


    <!-- http://ontology.ethereal.cz/irao/InformaticsResearchArtifact -->

    <owl:Class rdf:about="http://ontology.ethereal.cz/irao/InformaticsResearchArtifact">
        <rdfs:subClassOf rdf:resource="http://ontology.ethereal.cz/irao/ResearchArtifact"/>
        <rdfs:comment xml:lang="en">An informatics research artifact is a research artifact in the informatics field</rdfs:comment>
        <rdfs:isDefinedBy rdf:resource="http://ontology.ethereal.cz/irao"/>
        <rdfs:label xml:lang="en">Informatics Research Artifact</rdfs:label>
    </owl:Class>
    


    <!-- http://ontology.ethereal.cz/irao/License -->

    <owl:Class rdf:about="http://ontology.ethereal.cz/irao/License">
        <rdfs:comment xml:lang="en">A license authorizes the use, performace, or release of a research artifact</rdfs:comment>
        <rdfs:isDefinedBy rdf:resource="http://ontology.ethereal.cz/irao"/>
        <rdfs:label xml:lang="en">License</rdfs:label>
    </owl:Class>
    


    <!-- http://ontology.ethereal.cz/irao/LicenseType -->

    <owl:Class rdf:about="http://ontology.ethereal.cz/irao/LicenseType">
        <rdfs:comment xml:lang="en">The type of a license</rdfs:comment>
        <rdfs:isDefinedBy rdf:resource="http://ontology.ethereal.cz/irao"/>
        <rdfs:label xml:lang="en">License type</rdfs:label>
    </owl:Class>
    


    <!-- http://ontology.ethereal.cz/irao/Methodology -->

    <owl:Class rdf:about="http://ontology.ethereal.cz/irao/Methodology">
        <rdfs:subClassOf rdf:resource="http://ontology.ethereal.cz/irao/InformaticsResearchArtifact"/>
        <rdfs:comment xml:lang="en">Methodology is a type of research artifact</rdfs:comment>
        <rdfs:isDefinedBy rdf:resource="http://ontology.ethereal.cz/irao"/>
        <rdfs:label xml:lang="en">Methodology</rdfs:label>
    </owl:Class>
    


    <!-- http://ontology.ethereal.cz/irao/Middleware -->

    <owl:Class rdf:about="http://ontology.ethereal.cz/irao/Middleware">
        <rdfs:subClassOf rdf:resource="http://ontology.ethereal.cz/irao/Software"/>
        <rdfs:comment xml:lang="en">A middleware is a type of software that is used to connect software components in to a system</rdfs:comment>
        <rdfs:isDefinedBy rdf:resource="http://ontology.ethereal.cz/irao"/>
        <rdfs:label xml:lang="en">Middleware</rdfs:label>
    </owl:Class>
    


    <!-- http://ontology.ethereal.cz/irao/Model -->

    <owl:Class rdf:about="http://ontology.ethereal.cz/irao/Model">
        <rdfs:subClassOf rdf:resource="http://ontology.ethereal.cz/irao/InformaticsResearchArtifact"/>
        <rdfs:comment xml:lang="en">A model is a type of research artifact that can be used to describe other artifacts such as a dataset or a software</rdfs:comment>
        <rdfs:isDefinedBy rdf:resource="http://ontology.ethereal.cz/irao"/>
        <rdfs:label xml:lang="en">Model</rdfs:label>
    </owl:Class>
    


    <!-- http://ontology.ethereal.cz/irao/Ontology -->

    <owl:Class rdf:about="http://ontology.ethereal.cz/irao/Ontology">
        <rdfs:subClassOf rdf:resource="http://ontology.ethereal.cz/irao/DataModel"/>
        <rdfs:comment xml:lang="en">An ontology is a type of data model used to describe linked datasets</rdfs:comment>
        <rdfs:isDefinedBy rdf:resource="http://ontology.ethereal.cz/irao"/>
        <rdfs:label xml:lang="en">Ontology</rdfs:label>
    </owl:Class>
    


    <!-- http://ontology.ethereal.cz/irao/OntologyDesignPattern -->

    <owl:Class rdf:about="http://ontology.ethereal.cz/irao/OntologyDesignPattern">
        <rdfs:subClassOf rdf:resource="http://ontology.ethereal.cz/irao/InformaticsResearchArtifact"/>
        <rdfs:comment xml:lang="en">An ontology design pattern is a pattern used in designing ontologies</rdfs:comment>
        <rdfs:isDefinedBy rdf:resource="http://ontology.ethereal.cz/irao"/>
        <rdfs:label xml:lang="en">Ontology design pattern</rdfs:label>
    </owl:Class>
    


    <!-- http://ontology.ethereal.cz/irao/OpenStandard -->

    <owl:Class rdf:about="http://ontology.ethereal.cz/irao/OpenStandard">
        <rdfs:comment xml:lang="en">A open standard is a standard used to provide guidelines for the development and operations of artifacts and systems</rdfs:comment>
        <rdfs:isDefinedBy rdf:resource="http://ontology.ethereal.cz/irao"/>
        <rdfs:label xml:lang="en">Open Standard</rdfs:label>
    </owl:Class>
    


    <!-- http://ontology.ethereal.cz/irao/Protocol -->

    <owl:Class rdf:about="http://ontology.ethereal.cz/irao/Protocol">
        <rdfs:comment xml:lang="en">A protocol is used to provide guidelines to execute certain tasks</rdfs:comment>
        <rdfs:isDefinedBy rdf:resource="http://ontology.ethereal.cz/irao"/>
        <rdfs:label xml:lang="en">Protocol</rdfs:label>
    </owl:Class>
    


    <!-- http://ontology.ethereal.cz/irao/Publication -->

    <owl:Class rdf:about="http://ontology.ethereal.cz/irao/Publication">
        <rdfs:subClassOf rdf:resource="http://ontology.ethereal.cz/irao/ResearchOutput"/>
        <rdfs:comment xml:lang="en">A publication makes content and research results available to the general public via publication venues such as journals, books, websites, etc.</rdfs:comment>
        <rdfs:isDefinedBy rdf:resource="http://ontology.ethereal.cz/irao"/>
        <rdfs:label xml:lang="en">Publication</rdfs:label>
    </owl:Class>
    


    <!-- http://ontology.ethereal.cz/irao/Repository -->

    <owl:Class rdf:about="http://ontology.ethereal.cz/irao/Repository">
        <rdfs:comment xml:lang="en">A repository is an online storage for the deposit of research artifacts such as datasets and vocabularies</rdfs:comment>
        <rdfs:isDefinedBy rdf:resource="http://ontology.ethereal.cz/irao"/>
        <rdfs:label xml:lang="en">Repository</rdfs:label>
    </owl:Class>
    


    <!-- http://ontology.ethereal.cz/irao/RepositoryType -->

    <owl:Class rdf:about="http://ontology.ethereal.cz/irao/RepositoryType">
        <rdfs:comment xml:lang="en">A repository type can be a knowledge base, knowledge graph, version control hosting, etc.</rdfs:comment>
        <rdfs:isDefinedBy rdf:resource="http://ontology.ethereal.cz/irao"/>
        <rdfs:label xml:lang="en">Repository Type</rdfs:label>
    </owl:Class>
    


    <!-- http://ontology.ethereal.cz/irao/ResearchArtifact -->

    <owl:Class rdf:about="http://ontology.ethereal.cz/irao/ResearchArtifact">
        <rdfs:subClassOf rdf:resource="http://ontology.ethereal.cz/irao/ResearchOutput"/>
        <rdfs:comment xml:lang="en">A research artifact is a direct output or result of a research project</rdfs:comment>
        <rdfs:isDefinedBy rdf:resource="http://ontology.ethereal.cz/irao"/>
        <rdfs:label xml:lang="en">Research Artifact</rdfs:label>
    </owl:Class>
    


    <!-- http://ontology.ethereal.cz/irao/ResearchDomain -->

    <owl:Class rdf:about="http://ontology.ethereal.cz/irao/ResearchDomain">
        <rdfs:comment xml:lang="en">A research domain is the domain of interest of a research project</rdfs:comment>
        <rdfs:isDefinedBy rdf:resource="http://ontology.ethereal.cz/irao"/>
        <rdfs:label xml:lang="en">Research Domain</rdfs:label>
    </owl:Class>
    


    <!-- http://ontology.ethereal.cz/irao/ResearchField -->

    <owl:Class rdf:about="http://ontology.ethereal.cz/irao/ResearchField">
        <rdfs:comment xml:lang="en">A research field is the field of interest of a research project</rdfs:comment>
        <rdfs:isDefinedBy rdf:resource="http://ontology.ethereal.cz/irao"/>
        <rdfs:label xml:lang="en">Research Field</rdfs:label>
    </owl:Class>
    


    <!-- http://ontology.ethereal.cz/irao/ResearchOutput -->

    <owl:Class rdf:about="http://ontology.ethereal.cz/irao/ResearchOutput">
        <rdfs:comment xml:lang="en">A research output is the result of a research project</rdfs:comment>
        <rdfs:isDefinedBy rdf:resource="http://ontology.ethereal.cz/irao"/>
        <rdfs:label xml:lang="en">Research output</rdfs:label>
    </owl:Class>
    


    <!-- http://ontology.ethereal.cz/irao/ResearchProject -->

    <owl:Class rdf:about="http://ontology.ethereal.cz/irao/ResearchProject">
        <rdfs:subClassOf rdf:resource="http://vivoweb.org/ontology/core#Project"/>
        <rdfs:comment xml:lang="en">A research project is a project within the research domain with the endeavor of achieving scientific results</rdfs:comment>
        <rdfs:isDefinedBy rdf:resource="http://ontology.ethereal.cz/irao"/>
        <rdfs:label xml:lang="en">Research project</rdfs:label>
    </owl:Class>
    


    <!-- http://ontology.ethereal.cz/irao/Researcher -->

    <owl:Class rdf:about="http://ontology.ethereal.cz/irao/Researcher">
        <rdfs:subClassOf rdf:resource="http://xmlns.com/foaf/0.1/Person"/>
        <rdfs:comment xml:lang="en">A researcher is a person doing research</rdfs:comment>
        <rdfs:isDefinedBy rdf:resource="http://ontology.ethereal.cz/irao"/>
        <rdfs:label xml:lang="en">Researcher</rdfs:label>
    </owl:Class>
    


    <!-- http://ontology.ethereal.cz/irao/Service -->

    <owl:Class rdf:about="http://ontology.ethereal.cz/irao/Service">
        <rdfs:subClassOf rdf:resource="http://ontology.ethereal.cz/irao/Software"/>
        <rdfs:comment xml:lang="en">A service is a type of software that provides e.g. data or some type of functionalities</rdfs:comment>
        <rdfs:isDefinedBy rdf:resource="http://ontology.ethereal.cz/irao"/>
        <rdfs:label xml:lang="en">Service</rdfs:label>
    </owl:Class>
    


    <!-- http://ontology.ethereal.cz/irao/Software -->

    <owl:Class rdf:about="http://ontology.ethereal.cz/irao/Software">
        <rdfs:subClassOf rdf:resource="http://ontology.ethereal.cz/irao/InformaticsResearchArtifact"/>
        <rdfs:comment xml:lang="en">A software is a type of informatics research artifact</rdfs:comment>
        <rdfs:isDefinedBy rdf:resource="http://ontology.ethereal.cz/irao"/>
        <rdfs:label xml:lang="en">Software</rdfs:label>
    </owl:Class>
    


    <!-- http://ontology.ethereal.cz/irao/SoftwareFramework -->

    <owl:Class rdf:about="http://ontology.ethereal.cz/irao/SoftwareFramework">
        <rdfs:subClassOf rdf:resource="http://ontology.ethereal.cz/irao/Framework"/>
        <rdfs:comment xml:lang="en">A software framework is a type of software that provides guidelines for the development of new softwares</rdfs:comment>
        <rdfs:isDefinedBy rdf:resource="http://ontology.ethereal.cz/irao"/>
        <rdfs:label xml:lang="en">Software Framework</rdfs:label>
    </owl:Class>
    


    <!-- http://ontology.ethereal.cz/irao/SyntheticDataset -->

    <owl:Class rdf:about="http://ontology.ethereal.cz/irao/SyntheticDataset">
        <rdfs:subClassOf rdf:resource="http://ontology.ethereal.cz/irao/Dataset"/>
        <rdfs:comment xml:lang="en">Synthetic datasets are generated through computer programs, instead of being composed through the documentation of real-world events</rdfs:comment>
        <rdfs:isDefinedBy rdf:resource="http://ontology.ethereal.cz/irao"/>
        <rdfs:label xml:lang="en">Synthetic Dataset</rdfs:label>
    </owl:Class>
    


    <!-- http://ontology.ethereal.cz/irao/System -->

    <owl:Class rdf:about="http://ontology.ethereal.cz/irao/System">
        <rdfs:comment xml:lang="en">A system is a group of interacting or interrelated informatics components that form a unified whole</rdfs:comment>
        <rdfs:isDefinedBy rdf:resource="http://ontology.ethereal.cz/irao"/>
        <rdfs:label xml:lang="en">System</rdfs:label>
    </owl:Class>
    


    <!-- http://ontology.ethereal.cz/irao/Thesis -->

    <owl:Class rdf:about="http://ontology.ethereal.cz/irao/Thesis">
        <rdfs:subClassOf rdf:resource="http://ontology.ethereal.cz/irao/Publication"/>
        <rdfs:comment xml:lang="en">A thesis as a type of scientific or academic publication or dissertation is a document submitted in support of candidature for an academic degree or professional qualification presenting the author&apos;s research and findings</rdfs:comment>
        <rdfs:isDefinedBy rdf:resource="http://ontology.ethereal.cz/irao"/>
        <rdfs:label xml:lang="en">Thesis</rdfs:label>
    </owl:Class>
    


    <!-- http://ontology.ethereal.cz/irao/Vocabulary -->

    <owl:Class rdf:about="http://ontology.ethereal.cz/irao/Vocabulary">
        <rdfs:subClassOf rdf:resource="http://ontology.ethereal.cz/irao/InformaticsResearchArtifact"/>
        <rdfs:comment xml:lang="en">A vocabulary is used to provide a range of commonly used terms and their definitions</rdfs:comment>
        <rdfs:isDefinedBy rdf:resource="http://ontology.ethereal.cz/irao"/>
        <rdfs:label xml:lang="en">Vocabulary</rdfs:label>
    </owl:Class>
    


    <!-- http://ontology.ethereal.cz/irao/WebFramework -->

    <owl:Class rdf:about="http://ontology.ethereal.cz/irao/WebFramework">
        <rdfs:subClassOf rdf:resource="http://ontology.ethereal.cz/irao/SoftwareFramework"/>
        <rdfs:comment xml:lang="en">A web framework is a type of software framework that is used to develop applications on the web</rdfs:comment>
        <rdfs:isDefinedBy rdf:resource="http://ontology.ethereal.cz/irao"/>
        <rdfs:label xml:lang="en">Web Framework</rdfs:label>
    </owl:Class>
    


    <!-- http://ontology.ethereal.cz/irao/Workflow -->

    <owl:Class rdf:about="http://ontology.ethereal.cz/irao/Workflow">
        <rdfs:subClassOf rdf:resource="http://ontology.ethereal.cz/irao/InformaticsResearchArtifact"/>
        <rdfs:comment xml:lang="en">A workflow is a sequence of interrelated, orchestrated and repeatable tasks</rdfs:comment>
        <rdfs:isDefinedBy rdf:resource="http://ontology.ethereal.cz/irao"/>
        <rdfs:label xml:lang="en">Workflow</rdfs:label>
    </owl:Class>
    


    <!-- 
    ///////////////////////////////////////////////////////////////////////////////////////
    //
    // Individuals
    //
    ///////////////////////////////////////////////////////////////////////////////////////
     -->

    


    <!-- http://ontology.ethereal.cz/irao/accessibility#API -->

    <owl:NamedIndividual rdf:about="http://ontology.ethereal.cz/irao/accessibility#API">
        <rdf:type rdf:resource="http://ontology.ethereal.cz/irao/Accessibility"/>
        <rdfs:isDefinedBy rdf:resource="http://ontology.ethereal.cz/irao"/>
        <rdfs:label xml:lang="en">API</rdfs:label>
    </owl:NamedIndividual>
    


    <!-- http://ontology.ethereal.cz/irao/accessibility#Download -->

    <owl:NamedIndividual rdf:about="http://ontology.ethereal.cz/irao/accessibility#Download">
        <rdf:type rdf:resource="http://ontology.ethereal.cz/irao/Accessibility"/>
        <rdfs:isDefinedBy rdf:resource="http://ontology.ethereal.cz/irao"/>
        <rdfs:label xml:lang="en">Download</rdfs:label>
    </owl:NamedIndividual>
    


    <!-- http://ontology.ethereal.cz/irao/accessibility#OpenData -->

    <owl:NamedIndividual rdf:about="http://ontology.ethereal.cz/irao/accessibility#OpenData">
        <rdf:type rdf:resource="http://ontology.ethereal.cz/irao/Accessibility"/>
        <rdfs:isDefinedBy rdf:resource="http://ontology.ethereal.cz/irao"/>
        <rdfs:label xml:lang="en">Open Data</rdfs:label>
    </owl:NamedIndividual>
    


    <!-- http://ontology.ethereal.cz/irao/accessibility#OpenSource -->

    <owl:NamedIndividual rdf:about="http://ontology.ethereal.cz/irao/accessibility#OpenSource">
        <rdf:type rdf:resource="http://ontology.ethereal.cz/irao/Accessibility"/>
        <rdfs:isDefinedBy rdf:resource="http://ontology.ethereal.cz/irao"/>
        <rdfs:label xml:lang="en">Opensource</rdfs:label>
    </owl:NamedIndividual>
    


    <!-- http://ontology.ethereal.cz/irao/designquality#FAIR -->

    <owl:NamedIndividual rdf:about="http://ontology.ethereal.cz/irao/designquality#FAIR">
        <rdf:type rdf:resource="http://ontology.ethereal.cz/irao/DesignQuality"/>
        <rdfs:isDefinedBy rdf:resource="http://ontology.ethereal.cz/irao"/>
        <rdfs:label xml:lang="en">FAIR</rdfs:label>
    </owl:NamedIndividual>
    


    <!-- http://ontology.ethereal.cz/irao/designquality#Reuse -->

    <owl:NamedIndividual rdf:about="http://ontology.ethereal.cz/irao/designquality#Reuse">
        <rdf:type rdf:resource="http://ontology.ethereal.cz/irao/DesignQuality"/>
        <rdfs:isDefinedBy rdf:resource="http://ontology.ethereal.cz/irao"/>
        <rdfs:label xml:lang="en">Reuse</rdfs:label>
    </owl:NamedIndividual>
    


    <!-- http://ontology.ethereal.cz/irao/developmentstatus#alpha -->

    <owl:NamedIndividual rdf:about="http://ontology.ethereal.cz/irao/developmentstatus#alpha">
        <rdf:type rdf:resource="http://ontology.ethereal.cz/irao/DevelopmentStatus"/>
        <rdfs:isDefinedBy rdf:resource="http://ontology.ethereal.cz/irao"/>
        <rdfs:label xml:lang="en">Alpha</rdfs:label>
    </owl:NamedIndividual>
    


    <!-- http://ontology.ethereal.cz/irao/developmentstatus#beta -->

    <owl:NamedIndividual rdf:about="http://ontology.ethereal.cz/irao/developmentstatus#beta">
        <rdf:type rdf:resource="http://ontology.ethereal.cz/irao/DevelopmentStatus"/>
        <rdfs:isDefinedBy rdf:resource="http://ontology.ethereal.cz/irao"/>
        <rdfs:label xml:lang="en">Beta</rdfs:label>
    </owl:NamedIndividual>
    


    <!-- http://ontology.ethereal.cz/irao/developmentstatus#release -->

    <owl:NamedIndividual rdf:about="http://ontology.ethereal.cz/irao/developmentstatus#release">
        <rdf:type rdf:resource="http://ontology.ethereal.cz/irao/DevelopmentStatus"/>
        <rdfs:isDefinedBy rdf:resource="http://ontology.ethereal.cz/irao"/>
        <rdfs:label xml:lang="en">Release</rdfs:label>
    </owl:NamedIndividual>
    


    <!-- http://ontology.ethereal.cz/irao/openstandard#RDF -->

    <owl:NamedIndividual rdf:about="http://ontology.ethereal.cz/irao/openstandard#RDF">
        <rdf:type rdf:resource="http://ontology.ethereal.cz/irao/OpenStandard"/>
        <rdfs:isDefinedBy rdf:resource="http://ontology.ethereal.cz/irao"/>
        <rdfs:label xml:lang="en">RDF</rdfs:label>
    </owl:NamedIndividual>
    


    <!-- http://ontology.ethereal.cz/irao/openstandard#RDFS -->

    <owl:NamedIndividual rdf:about="http://ontology.ethereal.cz/irao/openstandard#RDFS">
        <rdf:type rdf:resource="http://ontology.ethereal.cz/irao/OpenStandard"/>
        <rdfs:isDefinedBy rdf:resource="http://ontology.ethereal.cz/irao"/>
        <rdfs:label xml:lang="en">RDFS</rdfs:label>
    </owl:NamedIndividual>
    


    <!-- http://ontology.ethereal.cz/irao/openstandard#SKOS -->

    <owl:NamedIndividual rdf:about="http://ontology.ethereal.cz/irao/openstandard#SKOS">
        <rdf:type rdf:resource="http://ontology.ethereal.cz/irao/OpenStandard"/>
        <rdfs:isDefinedBy rdf:resource="http://ontology.ethereal.cz/irao"/>
        <rdfs:label xml:lang="en">SKOS</rdfs:label>
    </owl:NamedIndividual>
    


    <!-- http://ontology.ethereal.cz/irao/openstandard#SPARQL -->

    <owl:NamedIndividual rdf:about="http://ontology.ethereal.cz/irao/openstandard#SPARQL">
        <rdf:type rdf:resource="http://ontology.ethereal.cz/irao/OpenStandard"/>
        <rdfs:isDefinedBy rdf:resource="http://ontology.ethereal.cz/irao"/>
        <rdfs:label xml:lang="en">SPARQL</rdfs:label>
    </owl:NamedIndividual>
    


    <!-- http://ontology.ethereal.cz/irao/openstandard#XML -->

    <owl:NamedIndividual rdf:about="http://ontology.ethereal.cz/irao/openstandard#XML">
        <rdf:type rdf:resource="http://ontology.ethereal.cz/irao/OpenStandard"/>
        <rdfs:isDefinedBy rdf:resource="http://ontology.ethereal.cz/irao"/>
        <rdfs:label xml:lang="en">XML</rdfs:label>
    </owl:NamedIndividual>
    


    <!-- http://ontology.ethereal.cz/irao/repositorytype#KnowledgeBase -->

    <owl:NamedIndividual rdf:about="http://ontology.ethereal.cz/irao/repositorytype#KnowledgeBase">
        <rdf:type rdf:resource="http://ontology.ethereal.cz/irao/RepositoryType"/>
        <rdfs:isDefinedBy rdf:resource="http://ontology.ethereal.cz/irao"/>
        <rdfs:label xml:lang="en">Knowledge base</rdfs:label>
    </owl:NamedIndividual>
    


    <!-- http://ontology.ethereal.cz/irao/repositorytype#VersionControlHosting -->

    <owl:NamedIndividual rdf:about="http://ontology.ethereal.cz/irao/repositorytype#VersionControlHosting">
        <rdf:type rdf:resource="http://ontology.ethereal.cz/irao/RepositoryType"/>
        <rdfs:isDefinedBy rdf:resource="http://ontology.ethereal.cz/irao"/>
        <rdfs:label xml:lang="en">Version control hosting</rdfs:label>
    </owl:NamedIndividual>
</rdf:RDF>



<!-- Generated by the OWL API (version 4.5.9.2019-02-01T07:24:44Z) https://github.com/owlcs/owlapi -->

